@prefix csv2rdf: <http://example.org/csv2rdf/> .
@prefix fdic: <http://example.org/fdic/> .
@prefix rdf: <http://www.w3.org/1999/02/22-rdf-syntax-ns#> .
@prefix rdfs: <http://www.w3.org/2000/01/rdf-schema#> .
@prefix xsd: <http://www.w3.org/2001/XMLSchema#> .
@prefix owl: <http://www.w3.org/2002/07/owl#> .
@prefix dcterms: <http://purl.org/dc/terms/> .
@prefix dcat: <http://www.w3.org/ns/dcat#> .
@prefix prov: <http://www.w3.org/ns/prov#> .
@prefix fibo: <https://spec.edmcouncil.org/fibo/ontology/> .
@prefix fibo-fbc: <https://spec.edmcouncil.org/fibo/ontology/FBC/> .
@prefix fibo-be: <https://spec.edmcouncil.org/fibo/ontology/BE/> .
@prefix fibo-fnd-plc-adr: <https://spec.edmcouncil.org/fibo/ontology/FND/Places/Addresses/> .
@prefix fibo-fnd-rel-rel: <https://spec.edmcouncil.org/fibo/ontology/FND/Relations/Relations/> .
@prefix geo: <http://www.opengis.net/ont/geosparql#> .
@prefix geonames: <http://www.geonames.org/ontology#> .
@prefix schema: <https://schema.org/> .
@prefix wgs84: <http://www.w3.org/2003/01/geo/wgs84_pos#> .
@prefix vcard: <http://www.w3.org/2006/vcard/ns#> .
@prefix foaf: <http://xmlns.com/foaf/0.1/> .
@prefix wikidata: <http://www.wikidata.org/entity/> .
@prefix dbpedia: <http://dbpedia.org/resource/> .



# X Coordinate Column
fdic:column_X a csv2rdf:ColumnAnnotation ;
    csv2rdf:columnName "X" ;
    rdfs:label "X Coordinate"@en ;
    dcterms:description "Longitude coordinate in decimal degrees" ;
    csv2rdf:dataType xsd:decimal ;
    rdfs:seeAlso geo:hasGeometry ,
                  wgs84:long ,
                  schema:longitude ,
                  <https://en.wikipedia.org/wiki/Longitude> ;
    owl:sameAs wikidata:Q34027 ; # Wikidata entity for longitude
    rdfs:comment "Maps to longitude in geographic coordinate system. X coordinate represents the east-west position"@en ;
    dcterms:references <https://www.w3.org/2003/01/geo/wgs84_pos#> .

# Y Coordinate Column
fdic:column_Y a csv2rdf:ColumnAnnotation ;
    csv2rdf:columnName "Y" ;
    rdfs:label "Y Coordinate"@en ;
    dcterms:description "Latitude coordinate in decimal degrees" ;
    csv2rdf:dataType xsd:decimal ;
    rdfs:seeAlso geo:hasGeometry ,
                  wgs84:lat ,
                  schema:latitude ,
                  <https://en.wikipedia.org/wiki/Latitude> ;
    owl:sameAs wikidata:Q34028 ; # Wikidata entity for latitude
    rdfs:comment "Maps to latitude in geographic coordinate system. Y coordinate represents the north-south position"@en ;
    dcterms:references <https://www.w3.org/2003/01/geo/wgs84_pos#> .

# Longitude Column
fdic:column_LONGITUDE a csv2rdf:ColumnAnnotation ;
    csv2rdf:columnName "LONGITUDE" ;
    rdfs:label "Longitude"@en ;
    dcterms:description "Geographic longitude" ;
    csv2rdf:dataType xsd:decimal ;
    rdfs:seeAlso geo:longitude ;
    owl:equivalentProperty geo:longitude .

# Latitude Column
fdic:column_LATITUDE a csv2rdf:ColumnAnnotation ;
    csv2rdf:columnName "LATITUDE" ;
    rdfs:label "Latitude"@en ;
    dcterms:description "Geographic latitude" ;
    csv2rdf:dataType xsd:decimal ;
    rdfs:seeAlso geo:latitude ;
    owl:equivalentProperty geo:latitude .

# Bank Name Column
fdic:column_NAME a csv2rdf:ColumnAnnotation ;
    csv2rdf:columnName "NAME" ;
    rdfs:label "Institution Name"@en ;
    dcterms:description "Legal name of financial institution" ;
    csv2rdf:dataType xsd:string ;
    rdfs:seeAlso <https://spec.edmcouncil.org/fibo/ontology/BE/LegalEntities/LegalPersons/hasLegalName> ,
                  fibo-fbc:FinancialInstitution ,
                  schema:BankOrCreditUnion ,
                  foaf:name ,
                  <https://www.investopedia.com/terms/f/financialinstitution.asp> ,
                  <https://en.wikipedia.org/wiki/Bank> ;
    owl:sameAs wikidata:Q22687 ; # Wikidata entity for bank
    rdfs:comment "The official legal name of the FDIC-insured institution as registered with regulatory authorities"@en ;
    dcterms:references dbpedia:Bank .

# Address Column
fdic:column_ADDRESS a csv2rdf:ColumnAnnotation ;
    csv2rdf:columnName "ADDRESS" ;
    rdfs:label "Street Address"@en ;
    dcterms:description "Physical street address of the institution" ;
    csv2rdf:dataType xsd:string ;
    rdfs:seeAlso fibo-fnd-plc-adr:StreetAddress ,
                  vcard:street-address ,
                  schema:streetAddress ,
                  <https://pe.usps.com/text/pub28/welcome.htm> ; # USPS Postal Addressing Standards
    rdfs:comment "Street address of the institution's physical location, formatted according to USPS standards"@en ;
    dcterms:conformsTo <https://www.usps.com/manage/forward-mail.htm> .

# City Column
fdic:column_CITY a csv2rdf:ColumnAnnotation ;
    csv2rdf:columnName "CITY" ;
    rdfs:label "City"@en ;
    dcterms:description "City name" ;
    csv2rdf:dataType xsd:string ;
    rdfs:seeAlso geonames:name ;
    rdfs:comment "City where the institution is located"@en .

# State Code Column
fdic:column_STALP a csv2rdf:ColumnAnnotation ;
    csv2rdf:columnName "STALP" ;
    rdfs:label "State Code"@en ;
    dcterms:description "State abbreviation" ;
    csv2rdf:dataType xsd:string ;
    rdfs:seeAlso geonames:stateCode ;
    rdfs:comment "Two-letter state abbreviation code"@en .

# State Name Column
fdic:column_STNAME a csv2rdf:ColumnAnnotation ;
    csv2rdf:columnName "STNAME" ;
    rdfs:label "State Name"@en ;
    dcterms:description "State name" ;
    csv2rdf:dataType xsd:string ;
    rdfs:seeAlso geonames:name ;
    rdfs:comment "Full name of the state"@en .

# ZIP Code Column
fdic:column_ZIP a csv2rdf:ColumnAnnotation ;
    csv2rdf:columnName "ZIP" ;
    rdfs:label "ZIP Code"@en ;
    dcterms:description "United States Postal Service ZIP code" ;
    csv2rdf:dataType xsd:string ;
    rdfs:seeAlso fibo-fnd-plc-adr:PostCodeIdentifier ,
                  vcard:postal-code ,
                  schema:postalCode ,
                  <https://tools.usps.com/go/ZipLookupAction> ,
                  <https://en.wikipedia.org/wiki/ZIP_Code> ;
    owl:sameAs wikidata:Q136208 ; # Wikidata entity for ZIP code
    rdfs:comment "5-digit Zone Improvement Plan (ZIP) postal code used by USPS for mail delivery"@en ;
    dcterms:conformsTo <https://pe.usps.com/cpim/ftp/pubs/Pub28/pub28.pdf> .

# FDIC Certificate Number Column
fdic:column_CERT a csv2rdf:ColumnAnnotation ;
    csv2rdf:columnName "CERT" ;
    rdfs:label "FDIC Certificate Number"@en ;
    dcterms:description "Unique FDIC-assigned certificate of insurance number" ;
    csv2rdf:dataType xsd:integer ;
    rdfs:seeAlso fibo-be:GovernmentIssuedLicense ,
                  fibo-fbc:RegulatoryLicense ,
                  schema:identifier ,
                  <https://www.fdic.gov/resources/bankers/call-reports/crinst-031/2019/2019-03-crinst-031-rc-a.pdf> ,
                  <https://en.wikipedia.org/wiki/Federal_Deposit_Insurance_Corporation#Certificate_numbers> ;
    owl:sameAs wikidata:Q116907062 ; # Wikidata property for FDIC certificate number
    rdfs:comment "Unique identifier assigned by the FDIC when granting deposit insurance. This number remains constant throughout the institution's existence"@en ;
    dcterms:issued "Federal Deposit Insurance Corporation" ;
    owl:equivalentClass [
        a owl:Restriction ;
        owl:onProperty dcterms:identifier ;
        owl:value "FDIC Certificate Number"^^xsd:string
    ] .

# Bank Class Column
fdic:column_BKCLASS a csv2rdf:ColumnAnnotation ;
    csv2rdf:columnName "BKCLASS" ;
    rdfs:label "Bank Classification"@en ;
    dcterms:description "Bank classification code" ;
    csv2rdf:dataType xsd:string ;
    rdfs:seeAlso <https://spec.edmcouncil.org/fibo/ontology/BE/Corporations/Corporations/OrganizationClassification> ;
    rdfs:comment "Classification code indicating the type of banking institution"@en .

# Service Type Description Column
fdic:column_SERVTYPE_DESC a csv2rdf:ColumnAnnotation ;
    csv2rdf:columnName "SERVTYPE_DESC" ;
    rdfs:label "Service Type Description"@en ;
    dcterms:description "Type of banking service provided" ;
    csv2rdf:dataType xsd:string ;
    rdfs:seeAlso <https://spec.edmcouncil.org/fibo/ontology/FND/ProductsAndServices/ProductsAndServices/Service> ;
    rdfs:comment "Description of the primary service type offered by the institution"@en .





# Resource documentation
fdic:CitedResources a owl:Class ;
    rdfs:label "Cited Resources"@en ;
    rdfs:comment "Documentation of external resources used for semantic mappings"@en .

fdic:FIBO_Resource a fdic:CitedResources ;
    rdfs:label "Financial Industry Business Ontology (FIBO)" ;
    dcterms:description "Industry-standard ontology for financial data developed by the EDM Council" ;
    foaf:homepage <https://spec.edmcouncil.org/fibo/> ;
    dcterms:source <https://github.com/edmcouncil/fibo> ;
    dcterms:type "Well-formed Ontology Standard" .

fdic:GeoSPARQL_Resource a fdic:CitedResources ;
    rdfs:label "OGC GeoSPARQL" ;
    dcterms:description "OGC standard for representing and querying geospatial data on the Semantic Web" ;
    foaf:homepage <https://opengeospatial.github.io/ogc-geosparql/geosparql11/geo.html> ;
    dcterms:type "Well-formed Ontology Standard" .

fdic:GeoNames_Resource a fdic:CitedResources ;
    rdfs:label "GeoNames Ontology" ;
    dcterms:description "Ontology for geographical database covering all countries" ;
    foaf:homepage <https://www.geonames.org/ontology/documentation.html> ;
    dcterms:type "Well-formed Ontology" .

fdic:SchemaOrg_Resource a fdic:CitedResources ;
    rdfs:label "Schema.org" ;
    dcterms:description "Collaborative vocabulary for structured data on the Internet" ;
    foaf:homepage <https://schema.org/> ;
    dcterms:type "Well-formed Vocabulary" .

fdic:Wikipedia_Resource a fdic:CitedResources ;
    rdfs:label "Wikipedia" ;
    dcterms:description "Open encyclopedia used for general concept definitions" ;
    foaf:homepage <https://en.wikipedia.org/> ;
    dcterms:type "Non-ontological Resource" .

fdic:Investopedia_Resource a fdic:CitedResources ;
    rdfs:label "Investopedia Financial Dictionary" ;
    dcterms:description "Comprehensive financial terms dictionary and educational resource" ;
    foaf:homepage <https://www.investopedia.com/dictionary/> ;
    dcterms:type "Non-ontological Resource" .



# Dataset metadata
fdic:FDICBankDataset a dcat:Dataset ;
    dcterms:title "FDIC-Insured Institutions Dataset" ;
    dcterms:description "Comprehensive dataset of FDIC-insured financial institutions in the United States, including location data, institutional identifiers, and service types" ;
    dcterms:publisher [
        a foaf:Organization ;
        foaf:name "Federal Deposit Insurance Corporation (FDIC)" ;
        foaf:homepage <https://www.fdic.gov/>
    ] ;
    dcat:keyword "banking", "financial institutions", "FDIC", "geospatial data", "US banks" ;
    dcterms:spatial [
        a dcterms:Location ;
        rdfs:label "United States of America"
    ] ;
    dcterms:temporal [
        a dcterms:PeriodOfTime ;
        rdfs:comment "Dataset is continuously updated"
    ] ;
    dcterms:conformsTo <https://spec.edmcouncil.org/fibo/ontology/> ,
                       <http://www.opengis.net/ont/geosparql#> ;
    prov:wasGeneratedBy [
        a prov:Activity ;
        rdfs:label "FDIC Data Collection and Reporting Process"
    ] .



# Column mapping class definition
csv2rdf:ColumnAnnotation a owl:Class ;
    rdfs:label "Column Mapping"@en ;
    rdfs:comment "A semantic mapping for a CSV column to ontological concepts"@en .

# Properties for column mappings
csv2rdf:columnName a owl:DatatypeProperty ;
    rdfs:label "column name"@en ;
    rdfs:domain csv2rdf:ColumnAnnotation ;
    rdfs:range xsd:string .

csv2rdf:dataType a owl:DatatypeProperty ;
    rdfs:label "data type"@en ;
    rdfs:comment "The expected data type of values in this column"@en ;
    rdfs:domain csv2rdf:ColumnAnnotation ;
    rdfs:range xsd:string .




# Ontology metadata
<http://example.org/csv2rdf/column-mappings> a owl:Ontology ;
    rdfs:label "CSV Column Mappings"@en ;
    dcterms:title "CSV Column Semantic Mappings"@en ;
    dcterms:description "Semantic mappings for CSV columns to established ontologies and resources"@en ;
    dcterms:created "2025-06-19"^^xsd:date ;
    dcterms:creator "Robust/FDIC_OMG" ;
    dcterms:license <https://creativecommons.org/licenses/by/4.0/> ;
    owl:imports <https://spec.edmcouncil.org/fibo/ontology/> ,
                <http://www.opengis.net/ont/geosparql#> ,
                <http://www.geonames.org/ontology#> ;
    rdfs:comment "This ontology provides comprehensive semantic mappings for FDIC CSV data columns to multiple ontologies and knowledge resources" .
